PFPL/Env.v
@@ -1,0 +1,188 @@
+Require Export Omega.
+Require Export List.
+Export ListNotations.
+
+Require Export Coq.Arith.Bool_nat.
+
+Definition Env A := list A.
+Definition Var   := nat.
+
+Definition getEnv {A} (env : Env A) n := nth_error env n.
+Definition InEnv {A} v t (env : Env A) := getEnv env v = Some t.
+
+Hint Unfold Env.
+Hint Unfold getEnv.
+Hint Unfold InEnv.
+
+Fixpoint insert {A} (env : Env A) v tv :=
+ match env,v with
+ | _, 0          => tv :: env
+ | [],      S v' => tv :: env
+ | (x::xs), S v' => x  :: insert xs v' tv
+ end.
+
+Lemma insert_0 {A} (env : Env A) t :
+      insert env 0 t = t :: env.
+Proof.
+ destruct env; auto.
+Qed.
+
+
+Lemma InEnv_app_end {A}
+  (env env' : Env A) t (v : Var) :
+  InEnv v t env -> InEnv v t (env ++ env').
+Proof.
+ unfold InEnv, getEnv.
+ revert env' v.
+ induction env; intros.
+  destruct v; simpl in H; inversion H.
+ destruct v.
+  auto.
+ simpl in H.
+ simpl.
+ eapply IHenv in H.
+ eassumption.
+Qed.
+
+
+Lemma InEnv_app_start {A}
+  (env env' : Env A) t (v : Var) :
+  InEnv v t env -> InEnv (length env' + v) t (env' ++ env).
+Proof.
+ unfold InEnv, getEnv.
+ revert v.
+ induction env'; intros.
+  simpl. assumption.
+ 
+ simpl.
+ apply IHenv' in H.
+ assumption.
+Qed.
+
+
+Lemma get_insert_lt {A} (env : Env A) i v ti tv :
+      InEnv i ti env ->
+      i < v ->
+      InEnv i ti (insert env v tv).
+Proof.
+ intros Hget Hlt.
+ revert v tv Hlt env Hget.
+ induction i; intros; unfold InEnv, getEnv in *.
+  destruct env. inversion Hget.
+  simpl in Hget. destruct v. omega.  
+ simpl. auto.
+ 
+ destruct env. inversion Hget.
+ simpl in Hget. destruct v. omega.
+ simpl.
+ apply IHi; try omega; auto.
+Qed.
+
+Lemma get_insert_ge {A} (env : Env A) i v ti tv :
+      InEnv i ti env ->
+      i >= v ->
+      InEnv (S i) ti (insert env v tv).
+Proof.
+ intros Hget Hge.
+ revert v tv env Hge Hget.
+ unfold InEnv, getEnv.
+ induction i; intros.
+
+ destruct env. inversion Hget.
+ simpl in Hget.
+ destruct v. simpl. assumption.
+ omega.
+ destruct env. inversion Hget.
+ destruct v. auto.
+ apply IHi.
+ omega.
+ assumption.
+Qed.
+
+Lemma uninsert {A} (t1 : A) e v t2:
+      insert (t1::e) (S v) t2 =
+      t1 :: (insert e v t2).
+Proof.
+ auto.
+Qed.
+
+
+Lemma InEnv_insert {A} (env : Env A) v t t':
+      InEnv v t' (insert env v t) ->
+      t = t'.
+Proof.
+ unfold InEnv, getEnv.
+ intros HIE. revert t t' env HIE.
+ induction v; intros.
+ destruct env; simpl in *; unfold value in *; congruence.
+ 
+ destruct env. simpl in *. destruct v; inversion HIE.
+ simpl in HIE.
+ apply IHv in HIE. assumption.
+Qed.
+
+
+
+Lemma insert_minus1 {A} (env : Env A) i v ti tv :
+      InEnv (S i) ti (insert env v tv) ->
+      S i > v ->
+      InEnv i ti env.
+Proof.
+ intros Hin Hge.
+ revert env v ti tv Hin Hge.
+ unfold InEnv, getEnv.
+ induction i; intros.
+ destruct v; destruct env; auto.
+ omega.
+
+ destruct env; destruct v; auto.
+ simpl.
+ eapply IHi.
+ simpl in Hin.
+ eassumption.
+ omega.
+Qed.
+
+
+Lemma insert_pre {A} (env : Env A) i v ti tv :
+      InEnv i ti (insert env v tv) ->
+      v <= length env ->
+      i < v ->
+      InEnv i ti env.
+Proof.
+ intros Hin Hlen Hge.
+ revert env v ti tv Hin Hge Hlen.
+ unfold InEnv, getEnv.
+ induction i; intros.
+ destruct v; destruct env; auto.
+ omega. omega. simpl in Hlen. omega.
+  
+
+ destruct env; destruct v; auto.
+ omega. simpl in Hlen. omega. omega.
+ simpl. 
+ eapply IHi.
+ simpl in Hin.
+ eassumption.
+ omega.
+ simpl in Hlen.
+ omega.
+Qed.
+
+
+
+
+Lemma InEnv_insert_n {A} (env : Env A) v t:
+      v <= length env ->
+      InEnv v t (insert env v t).
+Proof.
+ unfold InEnv, getEnv.
+ revert v t.
+ induction env; intros.
+ destruct v; auto. simpl in H. omega.
+ 
+ destruct v; auto.
+ simpl in *.
+ apply IHenv. omega.
+Qed.
+
