PFPL/ch6.v
@@ -1,0 +1,28 @@
+Require Import Env.
+
+Inductive Ty :=
+        | t_num   : Ty
+        | t_arrow : Ty -> Ty -> Ty.
+
+Definition Num := nat.
+
+Inductive Exp :=
+        | var    : Var -> Exp
+        | num    : Num -> Exp
+        | lambda : Ty  -> Exp -> Exp
+        | app    : Exp -> Exp -> Exp.
+(* does lambda need Ty? *)
+
+Definition TEnv := Env Ty.
+
+Inductive TYPE (env : TEnv) : Exp -> Ty -> Prop :=
+	| ty_env (v : Var) (t : Ty): (InEnv v t env) -> TYPE env (var v) t
+	| ty_num (n : Num) : TYPE env (num n) t_num
+	| ty_lambda (def body : Exp) (ty tbody : Ty) :
+		TYPE (ty :: env) body tbody ->
+		TYPE env (lambda ty body) (t_arrow ty tbody)
+	| ty_app (f x : Exp) (t1 t2 : Ty) :
+		TYPE env f (t_arrow t1 t2) ->
+		TYPE env x t1 ->
+		TYPE env (app f x) t2.
+
